Make reactor inputs and outputs lists instead of vectors.

src/determinism.lean
@@ -1,100 +1,178 @@
 import basic
 import data.vector
 
-namespace hidden 
+/- Reactor Primitives -/
 
-  variables i o : ℕ 
+-- A reactor's state fields and in-/output-ports are represented as lists of values with a fixed
+-- length. Single ports and state values can then be identified by an index into these lists.
+--! Using a `vector` makes reactors with different numbers of ports heterogenous, and therefore 
+--! un`list`able. Therefore `list` is currently used, which is not optimal.
+namespace reactor
 
-  def inputs := vector value i
-  def outputs := vector value o
-  def state := list value
+  def input  := list value
+  def output := list value
+  def state  := list value
 
-  -- REACTION
+end reactor
 
-  -- The output vector produced by a reaction contains ε for all of those ports which should remain unaffected.
-  def reaction := (inputs i × state) → (outputs o × state)
-  
-  namespace reaction
+/- Reaction -/
 
-    def determinism {i o : ℕ} (r : reaction i o) : Prop := 
-      ∀ is₁ is₂ : (inputs i × state), is₁ = is₂ → r is₁ = r is₂
+open reactor
 
-    theorem deterministic (r : reaction i o) : determinism r :=
-      assume is₁ is₂ : (inputs i × state),
-      assume h : is₁ = is₂,
-      show r is₁ = r is₂,
-      from congr_arg r h
+-- Given the current state and inputs, a reaction computes a new state and resulting outputs. 
+-- 
+-- Normally reactions are triggered upon a change to one of the input ports they depend on. In the
+-- current definition, this behavior is implicit (i.e. is moved into the reactions themselves).
+-- If a reaction wants to declare itself as non-dependent on the given inputs, it should output
+-- only `ε`s for the `outputs`, and keep the `state` unchanged. This will then be equivalent to not
+-- firing for the given input. 
+-- If the reaction *does* change `outputs` or `state`, it is considered to be dependent on the
+-- inputs that it used, and was therefore supposed to fire on their changing anyway. 
+-- The `outputs` produced by a reaction should contain `ε` for all ports which should remain 
+-- unaffected.
+--! Can a reaction write `ε` to an output port on purpose, to delete values written there by other
+--! reactions?
+def reaction := (input × state) → (output × state)
 
-  end reaction
+namespace reaction
 
-  -- BODY
+  -- A reaction is deterministic, if given equal inputs, it produces equal outputs.
+  -- Since reactions are functions, determinism is trivially fulfilled.
+  theorem deterministic (r : reaction) (is₁ is₂ : input × state) :
+    is₁ = is₂ → r is₁ = r is₂ := 
+    assume h : is₁ = is₂,
+    congr_arg r h
 
-  -- The order produced by a body only describes the *priority* of the reactions, not their connections.
-  inductive body
-    | single (r : reaction i o) : body
-    | composed (head : reaction i o) (tail : body) : body
+end reaction
 
-  namespace body
+/- Reactor Precedence List -/
 
-    private def merge {o : ℕ} (o₁ o₂ : outputs o) : outputs o := sorry
+namespace reactor
 
-    private def process' {i o : ℕ} : (inputs i × outputs o × state) → (body i o) → (outputs o × state)
-      | ios (body.single r)     := let os := r ⟨ios.1, ios.2.2⟩ in ⟨merge os.1 ios.2.1, os.2⟩ 
-      | ios (body.composed r t) := let os := r ⟨ios.1, ios.2.2⟩ in let os' := process' ⟨ios.1, os.1, os.2⟩ t in ⟨merge os.1 os'.1, os'.2⟩ 
+  -- In this simple model of reactors, precendece between reactions arises *only* from an explicit
+  -- ordering (not reactor-internal dependencies). The precedence *graph* therefore collapses to a
+  -- *list* which codifies the order implicitly.
+  -- The list is also used as the means of collecting all of the reactions of a reactor.
+  -- An own type is chosen over `list`, to disallow empty lists.
+  inductive precedence_list
+    | single (r : reaction) : precedence_list
+    | chain (first : reaction) (later : precedence_list) : precedence_list
 
-    def process {i o : ℕ} : (inputs i × state) → (body i o) → (outputs o × state)
-      | is (body.single r)     := r is
-      | is (body.composed r t) := let os := r is in process' ⟨is.1, os.1, os.2⟩ t
+  namespace precedence_list
 
-    def determinism {i o : ℕ} (b : body i o) : Prop := 
-      ∀ is₁ is₂ : (inputs i × state), is₁ = is₂ → (process is₁ b) = (process is₂ b)
+    -- Merges two outputs in such a way that all of the non-`ε` values of `o₁` override the values
+    -- in `o₂`.
+    private def merge (o₁ o₂ : output) : output := sorry
 
-    theorem deterministic (b : body i o) : determinism b :=
-      assume is₁ is₂ : (inputs i × state),
-      assume h : is₁ = is₂,
-      show process is₁ b = process is₂ b,
-      from congr (congr_arg process h) (refl b)
+    -- Cf. `process`.
+    private def process' : (input × output × state) → (precedence_list) → (output × state)
+      | ios (single r)  := let os := r ⟨ios.1, ios.2.2⟩ in 
+                           ⟨merge os.1 ios.2.1, os.2⟩ 
+      | ios (chain f l) := let os := f ⟨ios.1, ios.2.2⟩ in
+                           let os' := process' ⟨ios.1, os.1, os.2⟩ l in
+                           ⟨merge os.1 os'.1, os'.2⟩ 
 
-  end body
+    -- Basic reactions process their input directly, since they are functions. A collection 
+    -- (precedence-list) of reactions uses the following mechanism, to go from input to singular
+    -- final output.
+    -- Reactions were defined as functions that only change the state or return outputs different
+    -- from `ε`s (cf. `reaction`) *if* they consider themselves to be dependent on the given input.
+    -- In turn, to compute the result of a collection of reactions for a given input, the input can
+    -- simply be fed through the precendence list, from one reaction to the next.
+    -- If a reaction changes the state, this updated state will be passed along to the next
+    -- reaction.
+    -- If a reaction produces output, this output will be merged onto a cumulative outputs-value
+    -- that is carried along the processing-chain (cf. `process'`).
+    -- If a reaction is definitionally considered to not trigger on the given input, its output
+    -- will change neither the state- nor outputs-value that is carried along the processing-chain.
+    -- To implement this functionality, a seperate `process'` function is used, that can carry the
+    -- outputs.
+    def process : (input × state) → (precedence_list) → (output × state)
+      | is (single r)  := r is
+      | is (chain f l) := let os := f is in
+                          process' ⟨is.1, os.1, os.2⟩ l
 
-  -- SEQUENCE
+    -- A collection (precendence-list) of reactions is deterministic, if given equal inputs, the
+    -- results of processing them is equal. 
+    -- Since `process` is a function, determinism is trivially fulfilled.
+    theorem deterministic (p : precedence_list) (is₁ is₂ : input × state) : 
+      is₁ = is₂ → (process is₁ p) = (process is₂ p) :=
+      assume h : is₁ = is₂, 
+      congr (congr_arg process h) (refl p)
 
-  namespace sequence
+  end precedence_list
+
+/- Sequential Processing -/
+
+namespace reactor
+
+  namespace sequential
     
-    -- Given a list of inputs, an initial state and a body, `process` computes the resulting state and outputs.
-    def process {i o : ℕ} : list (inputs i) → (state) → (body i o) → list (outputs o × state)
+    -- Given a list of inputs, an initial state and a collection of reactions, `process` computes the
+    -- result (state and outputs) of processing the inputs sequentially, starting in the given state.
+    -- Any outputs and changes to the state produced along the way. are captured in the resulting
+    -- list.
+    -- This is akin to `reactor.precedence_list.process`, with the difference being that (a) the
+    -- basic unit of processing is now an entire precende-list (that is used repeatedly) instead of
+    -- just single reactions and (b) the outputs are listed individually rather than merged. The 
+    -- state is passed along from iteration to iteration though, just like before.
+    def process : list input → state → precedence_list → list (output × state)
       | [] _ _ := []
-      | (list.cons i_h i_t) s b := let os' := body.process ⟨i_h, s⟩ b in list.cons os' (process i_t os'.2 b) 
+      | (list.cons i_h i_t) s b := let os' := precedence_list.process ⟨i_h, s⟩ b in
+                                   list.cons os' (process i_t os'.2 b) 
 
-    def determinism {i o : ℕ} (b : body i o) : Prop := 
-      ∀ (i₁ i₂ : list (inputs i)) (s₁ s₂ : state), 
-      (i₁ = i₂ ∧ s₁ = s₂) → (process i₁ s₁ b) = (process i₂ s₂ b)
-
-    theorem deterministic (b : body i o) : determinism b :=
-      assume i₁ i₂ : list (inputs i),
-      assume s₁ s₂ : state,
+    -- Processing a sequential input to a collection of reactions is deterministic, if given equal 
+    -- inputs, the results of processing them is equal. 
+    -- Since `process` is a function, determinism is trivially fulfilled.
+    theorem deterministic (p : precedence_list) (i₁ i₂ : list input) (s₁ s₂ : state) :
+      (i₁ = i₂ ∧ s₁ = s₂) → (process i₁ s₁ p) = (process i₂ s₂ p) :=
       assume h : i₁ = i₂ ∧ s₁ = s₂,
-      show process i₁ s₁ b = process i₂ s₂ b, 
-      from congr (congr (congr_arg process h.left) h.right) (refl b)
+      congr (congr (congr_arg process h.left) h.right) (refl p)
 
-  end sequence
+  end sequential
 
-  -- REACTOR
+end reactor
 
-  structure reactor :=
-    (in_ports : inputs i)
-    (out_ports : outputs o)
-    (s : state)
-    (b : body i o)
+/- Reactor -/
 
-  -- NETWORK
+-- At any given time a reactor has values (or lack thereof via `ε`) for its input and output ports
+-- as well as its state. The processing of values is performed by its reactions, which should only
+-- ever receive the reactor's own input values and state as input. The result of processing should
+-- only ever be written back to the reactor itself.
+structure reactor :=
+  («input» : input)
+  («output» : output)
+  («state» : state)
+  (reactions : precedence_list)
 
-  -- By defining the `reactors` as a list instead of a set, we can again drop the need for identifiers and use the index
-  -- into the list as a reactor's identifier.
-  --
-  -- The list needs to be homogenous over the type of rectors wrt. `i o`. Is this possible?
+namespace reactor 
+
+  -- Processing a computation for a single unconnected reactor consists of (1) processing its input
+  -- and state through its reactions (2) writing the resulting output and state back to the reactor
+  -- and (3) wiping the reactor's input (setting them all to `ε`).
+  def process (r : reactor) : reactor :=
+    let os := precedence_list.process ⟨r.input, r.state⟩ r.reactions in
+    let i' := sorry in -- Make a list of `r.input.length` many `ε`s.
+    ⟨i', os.1, os.2, r.reactions⟩ 
+
+  -- Processing a computation of a single unconnected reactor is deterministic, if given equal
+  -- inputs, the resulting reactors are equal. 
+  -- Since `process` is a function, determinism is trivially fulfilled.
+  theorem deterministic (r₁ r₂ : reactor) : 
+    r₁ = r₂ → process r₁ = process r₂ :=
+    assume h : r₁ = r₂,
+    congr_arg process h
+
+end reactor
+
+/- Reactor Network -/
+
+namespace reactor 
+
+  -- By defining the `reactors` as a list instead of a set, we remove the need for identifiers and
+  -- use the index into the list as a reactor's identifier.
   structure network :=
-    (reactors : list (reactor i o))
-    (connections : (reactor i o) × ℕ → (reactor i o) × ℕ)
+    (reactors : list reactor)
+    (connections: (ℕ × ℕ) → (ℕ × ℕ))
 
-end hidden
+end reactor
